function calls and procedures

While.thy
@@ -12,12 +12,22 @@ text {*
 
 notation Id_on ("\<lfloor>_\<rfloor>" 100) (* relations below the identity form tests *)  
 
+type_synonym ('v, 's) lval = "('v \<Rightarrow> 'v) \<Rightarrow> 's \<Rightarrow> 's"
+type_synonym ('v, 's) rval = "'s \<Rightarrow> 'v"
+type_synonym ('v, 's) var = "('v, 's) lval \<times> ('v, 's) rval"
+
 definition abort :: "'s rel" ("abort") where "abort \<equiv> {}"
 
 definition skip :: "'s rel" ("skip") where "skip \<equiv> Id" 
 
-definition to_rel :: "('s \<Rightarrow> 's) \<Rightarrow> 's rel" ("\<langle>_\<rangle>" 100) where
+definition graph :: "('s \<Rightarrow> 's) \<Rightarrow> 's rel" ("\<langle>_\<rangle>" 100) where
   "\<langle>f\<rangle> \<equiv> {(s, f s) | s. True}"
+
+definition subst :: "'s set \<Rightarrow> ('v, 's) lval \<Rightarrow> ('v, 's) rval \<Rightarrow> 's set" where
+  "subst P u_upd t \<equiv> Collect (\<lambda>s. u_upd (\<lambda>_. t s) s \<in> P)"
+
+definition assign :: "('v, 's) lval \<Rightarrow> ('s \<Rightarrow> 'v) \<Rightarrow> 's rel" where
+  "assign u_upd t \<equiv> \<langle>\<lambda>s. u_upd (\<lambda>_. t s) s\<rangle>"
 
 definition seq :: "'s rel \<Rightarrow> 's rel \<Rightarrow> 's rel" (infixr ";" 60) where
   "seq \<equiv> relcomp"
@@ -25,24 +35,35 @@ definition seq :: "'s rel \<Rightarrow> 's rel \<Rightarrow> 's rel" (infixr ";"
 definition cond :: "'s set \<Rightarrow> 's rel \<Rightarrow> 's rel \<Rightarrow> 's rel" where
   "cond b x y \<equiv> (\<lfloor>b\<rfloor>;x) \<union> (\<lfloor>-b\<rfloor>;y)"
 
-definition while :: "'s set \<Rightarrow> 's rel \<Rightarrow> 's rel" where
-  "while b x \<equiv> (\<lfloor>b\<rfloor>;x)\<^sup>*; \<lfloor>-b\<rfloor>"
+definition cwhile :: "'s set \<Rightarrow> 's rel \<Rightarrow> 's rel" where
+  "cwhile b x \<equiv> (\<lfloor>b\<rfloor>;x)\<^sup>*; \<lfloor>-b\<rfloor>"
 
 definition dyn :: "('s \<Rightarrow> 's rel) \<Rightarrow> 's rel" ("\<lceil>_\<rceil>" 100) where
   "\<lceil>g\<rceil> \<equiv> {(s, s'). (s, s') \<in> g s}"
-  
-definition loc :: "'s rel \<Rightarrow> ('s \<Rightarrow> 's rel) \<Rightarrow> 's rel" where
-  "loc x upd \<equiv> \<lceil>\<lambda>s. x; upd s \<rceil>"
 
-definition block :: "('s \<Rightarrow> 's) \<Rightarrow> 's rel \<Rightarrow> ('s \<Rightarrow> 's \<Rightarrow> 's) \<Rightarrow> ('s \<Rightarrow> 's \<Rightarrow> 's rel) \<Rightarrow> 's rel" where
-  "block init x ret c \<equiv> \<lceil>\<lambda>s. \<langle>init\<rangle>; x; \<lceil>\<lambda>t. \<langle>ret s\<rangle>; c s t\<rceil> \<rceil>"
+definition block :: "'s rel \<Rightarrow> ('s \<Rightarrow> 's \<Rightarrow> 's) \<Rightarrow> 's rel" where
+  "block x ret \<equiv> \<lceil>\<lambda>s. x; \<langle>ret s\<rangle>\<rceil>"
+
+definition loc_block :: "('v, 's) lval \<Rightarrow> ('v, 's) rval \<Rightarrow> ('v, 's) rval \<Rightarrow> 's rel \<Rightarrow> 's rel" where
+  "loc_block z_upd z t x \<equiv> (block (\<langle>\<lambda>s. z_upd (\<lambda>_. t s) s\<rangle>; x) (\<lambda>s. z_upd (\<lambda>_. z s)))"
+
+type_synonym ('v, 's) func = "('s rel \<times> ('v, 's) rval)"
+
+abbreviation fun_block :: "'s rel \<Rightarrow> ('v, 's) rval \<Rightarrow> ('v, 's) func" where
+  "fun_block R y \<equiv> (R, y)"
+
+abbreviation proc_block :: "('v, 's) func \<Rightarrow> 's rel" ("proc _") where
+  "proc_block \<equiv> fst"
+
+definition fun_call :: "('v, 's) lval \<Rightarrow> ('v, 's) func \<Rightarrow> 's rel" where
+  "fun_call u_upd F \<equiv> block (fst F) (\<lambda>s t. u_upd (\<lambda>_. snd F t) t)"
   
 text {* Annotated programs for automatic verification *}
 
-definition awhile :: "'s set\<Rightarrow> 's set \<Rightarrow> 's rel \<Rightarrow> 's rel" where
-  "awhile i b x \<equiv> while b x"
+definition awhile :: "'s set \<Rightarrow> 's set \<Rightarrow> 's rel \<Rightarrow> 's rel" where
+  "awhile i b x \<equiv> cwhile b x"
 
-definition apre :: "'s set\<Rightarrow> 's rel \<Rightarrow> 's rel" where
+definition apre :: "'s set \<Rightarrow> 's rel \<Rightarrow> 's rel" where
   "apre p x \<equiv> x"
 
 definition apost :: "'s rel \<Rightarrow> 's set\<Rightarrow> 's rel" where
@@ -50,5 +71,6 @@ definition apost :: "'s rel \<Rightarrow> 's set\<Rightarrow> 's rel" where
 
 definition aprog :: "'s set\<Rightarrow> 's rel \<Rightarrow> 's set\<Rightarrow> 's rel" where
   "aprog p x q \<equiv> x"
+
 
 end
