Hoare.thy
@@ -10,21 +10,35 @@ no_notation comp_op ("n_" [90] 91)
   
 notation inf (infixl "\<sqinter>" 60)
 
+(***********************************************************************************************)
+
+text {* Verification condition generator *}
+
 named_theorems hl_rules
 
 method hoare_step uses simp declares hl_rules = (
-  ((rule allI | rule ballI | subst simp)+)?;
+  ((rule allI | rule ballI | subst simp | subst fst_conv)+)?;
   (assumption | rule subset_refl | rule hl_rules)
 )
 
 method hoare uses simp declares hl_rules = 
-  (hoare_step; hoare?)+
+  (hoare_step simp: simp hl_rules: hl_rules; hoare?)+
 
 method hoarerule uses first simp declares hl_rules = 
   (((rule allI | rule ballI | subst simp)+)?, rule first; hoare?)
 
+(***********************************************************************************************)
+
+text {* Classic Hoare logic *}
+
 definition ht :: "'s set \<Rightarrow> 's rel \<Rightarrow> 's set \<Rightarrow> bool" where
   "ht P x Q \<equiv> \<lfloor>P\<rfloor>;x \<subseteq> x;\<lfloor>Q\<rfloor>"
+
+lemma ht_true [intro]: "ht P x UNIV"
+  by (auto simp: ht_def seq_def)
+
+lemma hl_false [intro]: "ht {} x Q"
+  by (auto simp: ht_def seq_def)
 
 lemma hl_abort [hl_rules]: "ht P abort Q"
   by (auto simp: ht_def abort_def seq_def)
@@ -32,8 +46,11 @@ lemma hl_abort [hl_rules]: "ht P abort Q"
 lemma hl_skip [hl_rules]: "P \<subseteq> Q \<Longrightarrow> ht P skip Q"
   by (auto simp: ht_def skip_def seq_def)
   
-lemma hl_to_rel [hl_rules]: "P \<subseteq> {s. f s \<in> Q} \<Longrightarrow> ht P (\<langle>f\<rangle>) Q"
-  by (auto simp: ht_def to_rel_def seq_def)
+lemma hl_graph [hl_rules]: "P \<subseteq> {s. f s \<in> Q} \<Longrightarrow> ht P (\<langle>f\<rangle>) Q"
+  by (auto simp: ht_def graph_def seq_def)
+
+lemma hl_assign [hl_rules]: "P \<subseteq> subst Q z_upd t \<Longrightarrow> ht P (assign z_upd t) Q"
+  by (auto simp: assign_def subst_def intro: hl_graph)
 
 lemma hl_seq [hl_rules]: "ht R y Q \<Longrightarrow> ht P x R \<Longrightarrow> ht P (x; y) Q"
   by (force simp: ht_def seq_def)
@@ -44,11 +61,11 @@ lemma hl_split: "ht P x {t. Q t} \<Longrightarrow> ht P x {t. Q' t} \<Longrighta
 lemma hl_cond : "ht (b \<sqinter> P) x Q \<Longrightarrow> ht (-b \<sqinter> P) y Q \<Longrightarrow> ht P (cond b x y) Q"
   by (fastforce simp: ht_def cond_def seq_def)
 
-lemma hl_cond_tac [hl_rules]: "P \<subseteq> P' \<union> - b \<Longrightarrow> P \<subseteq> P''  \<union> b  \<Longrightarrow> ht P' x Q \<Longrightarrow> ht P'' y Q \<Longrightarrow> ht P (cond b x y) Q"
+lemma hl_cond_aux [hl_rules]: "P \<subseteq> (P' \<union> - b) \<inter> (P'' \<union> b)  \<Longrightarrow> ht P' x Q \<Longrightarrow> ht P'' y Q \<Longrightarrow> ht P (cond b x y) Q"
   by (fastforce simp: ht_def cond_def seq_def)
   
-lemma hl_while: "ht (b \<sqinter> i) x i \<Longrightarrow> ht i (while b x) (-b \<sqinter> i)"
-proof (simp add: ht_def while_def seq_def)
+lemma hl_while: "ht (b \<sqinter> i) x i \<Longrightarrow> ht i (cwhile b x) (-b \<sqinter> i)"
+proof (simp add: ht_def cwhile_def seq_def)
   assume "\<lfloor>b \<sqinter> i\<rfloor> O x \<subseteq> x O \<lfloor>i\<rfloor>"
   hence "\<lfloor>i\<rfloor> O (\<lfloor>b\<rfloor> O x)\<^sup>* \<subseteq> (\<lfloor>b\<rfloor> O x)\<^sup>* O \<lfloor>i\<rfloor>"
     by (force intro!: rel_kat.star_sim2)
@@ -56,8 +73,9 @@ proof (simp add: ht_def while_def seq_def)
     by auto
 qed
 
-lemma hl_dyn [hl_rules]: "\<forall>s \<in> P. ht P (g s) Q \<Longrightarrow> ht P (\<lceil>g\<rceil>) Q"
-  by (fastforce simp: ht_def seq_def dyn_def)
+(***********************************************************************************************)
+
+text {* Weakening / Strengthening / Consequence Rules *}
 
 lemma hl_pre: "P \<le> P' \<Longrightarrow> ht P' x Q \<Longrightarrow> ht P x Q"
   by (fastforce simp: ht_def le_fun_def seq_def)
@@ -68,71 +86,70 @@ lemma hl_post: "Q' \<le> Q \<Longrightarrow> ht P x Q' \<Longrightarrow> ht P x 
 lemma hl_classic: "P \<le> P' \<Longrightarrow> Q' \<le> Q \<Longrightarrow> ht P' x Q' \<Longrightarrow> ht P x Q"
   by (fastforce simp: ht_def le_fun_def seq_def)
   
-lemma hl_conseq: "\<forall>s. ht (P' s) c (Q' s) \<Longrightarrow> \<forall>s. s \<in> P \<longrightarrow> (\<exists>s'. s \<in> P' s' \<and> (Q' s' \<subseteq> Q)) \<Longrightarrow> ht P c Q"
+lemma hl_conseq: "\<forall>z. ht (P' z) c (Q' z) \<Longrightarrow> \<forall>s. s \<in> P \<longrightarrow> (\<exists>z. s \<in> P' z \<and> (Q' z \<subseteq> Q)) \<Longrightarrow> ht P c Q"
   by (force simp: ht_def seq_def)
 
-lemma hl_block [hl_rules]: "P \<subseteq> {s. init s \<in> P' s} \<Longrightarrow> \<forall>s. ht (P' s) x {t. ret s t \<in> R s t}
-  \<Longrightarrow> \<forall>s t. ht (R s t) (c s t) Q \<Longrightarrow> ht P (block init x ret c) Q"
-  apply (rule hl_conseq [where P'="\<lambda>s'. {s. s = s' \<and> init s \<in> P' s'}" and Q'="\<lambda> s'. Q"])
-  apply (hoare_step simp: block_def, hoare_step)
-  apply (rule_tac R="{t. ret s t \<in> R s t}" in hl_seq)
-  apply (rule_tac P'="\<lambda>s'. {t. t=s' \<and> ret s t \<in> R s t}" and Q'="\<lambda>s'. Q" in hl_conseq)
-  apply hoare
-  apply (erule_tac x=sa in allE, erule_tac x=sc in allE, assumption)
-  apply force
-  apply force
-  apply (erule_tac x=s in allE, assumption)
-  apply hoare_step
-  apply force+
- done
+lemma hl_kleymann: "\<forall>z. ht (P' z) x (Q' z) \<Longrightarrow> \<forall>s t. (\<forall>z. s \<in> P' z \<longrightarrow> t \<in> Q' z) \<longrightarrow> (\<forall>z. s \<in> P z \<longrightarrow> t \<in> Q z) \<Longrightarrow> \<forall>z. ht (P z) x (Q z)"
+  by (fastforce simp: apre_def seq_def ht_def)
 
-lemma ht_true [intro]: "ht UNIV x UNIV"
-  by (auto simp: ht_def seq_def)
+(***********************************************************************************************)
 
-lemma hl_false [intro]: "ht {} x {}"
-  by (auto simp: ht_def seq_def)
+text {* Blocks / Procedures / Recursive Calls *}
 
-lemma hl_Sup: "\<forall>x \<in> X. ht P x Q \<Longrightarrow> ht P (Sup X) Q"
+lemma hl_dyn [hl_rules]: "\<forall>s \<in> P. ht P (g s) Q \<Longrightarrow> ht P (\<lceil>g\<rceil>) Q"
+  by (fastforce simp: ht_def seq_def dyn_def)
+
+lemma hl_local_inv: "\<forall>s s'. z (z_upd (\<lambda>_. z s) s') = z s \<Longrightarrow> P \<le> {s. z s = u} \<Longrightarrow> ht P (loc_block z_upd z t x) {s. z s = u }"
+  by (auto simp: block_def loc_block_def graph_def dyn_def seq_def ht_def)
+
+lemma hl_block: "\<forall>s. ht P x {t. ret s t \<in> Q} \<Longrightarrow> ht P (block x ret) Q"
+  by (hoare simp: block_def) force
+
+lemma hl_loc_block: "\<forall>s. ht P (\<langle>\<lambda>s. z_upd (\<lambda>_. t s) s\<rangle>; x) {t. z_upd s t \<in> Q} \<Longrightarrow> ht P (loc_block z_upd z t x) Q"
+  by (auto simp: loc_block_def intro: hl_block)
+
+lemma hl_fun_block [hl_rules]: "ht P R (subst Q z_upd y) \<Longrightarrow> ht P (fun_call z_upd (R, y)) Q"
+  by (auto simp: fun_call_def subst_def intro: hl_block)
+
+lemma hl_Sup: "\<forall>x \<in> X. \<forall>z. ht (P z) (x z) (Q z) \<Longrightarrow> \<forall>z. ht (P z) (Sup X z) (Q z)"
   by (fastforce simp: ht_def seq_def)
-thm allE
-lemma hl_rec [hl_rules]: "mono f \<Longrightarrow> (\<And>x. \<forall>z. ht (P z) x (Q z) \<Longrightarrow> \<forall>z. ht (P z) (f x) (Q z)) \<Longrightarrow> \<forall>z. ht (P z) (lfp f) (Q z)"
 
-  apply (rule lfp_ordinal_induct)
-apply simp
-apply force
-apply (auto intro: hl_Sup)
-done
+lemma hl_rec [hl_rules]: "mono f \<Longrightarrow> (\<And>x. \<forall>z. ht (P z) (x z) (Q z) \<Longrightarrow> \<forall>z. ht (P z) (f x z) (Q z)) \<Longrightarrow> \<forall>z. ht (P z) (lfp f z) (Q z)"
+  apply (erule lfp_ordinal_induct [where f=f], simp)
+  by (force intro!: hl_Sup)
 
-lemma hl_rec2 [hl_rules]: "mono f \<Longrightarrow> (\<And>x. \<forall>z. ht (P z) x (Q z) \<Longrightarrow> \<forall>z. ht (P z) (f z x) (Q z)) \<Longrightarrow> \<forall>z. ht (P z) (lfp (f z)) (Q z)"
-sorry
+(***********************************************************************************************)
 
 text {* Annotated programs *}
 
 lemma hl_awhile [hl_rules]: "P \<subseteq> i \<Longrightarrow> -b \<inter> i \<subseteq> Q \<Longrightarrow> ht (b \<sqinter> i) x i \<Longrightarrow> ht P (awhile i b x) Q"
   by (hoarerule simp: awhile_def first: hl_conseq hl_rules: hl_while) force
   
-lemma hl_apre: "P \<subseteq> P' \<Longrightarrow> ht P' x Q \<Longrightarrow> ht P (apre P' x) Q"
+lemma hl_apre_classic: "P \<le> P' \<Longrightarrow> ht P' x Q \<Longrightarrow> ht P (apre P' x) Q"
   by (hoarerule simp: apre_def first: hl_pre)
 
-lemma hl_apre2: "\<forall>z. ht (P' z) x (Q' z) \<Longrightarrow> \<forall>s t. (\<forall>z. s \<in> P' z \<longrightarrow> t \<in> Q' z) \<longrightarrow> (\<forall>z. s \<in> P z \<longrightarrow> t \<in> Q z) \<Longrightarrow> \<forall>z. ht (P z) x (Q z)"
-  apply (simp add: apre_def seq_def ht_def)
-  apply auto
-  by force
+lemma hl_apre_kleymann_aux: "\<forall>z. ht (P' z) x (Q z) \<Longrightarrow> \<forall>s t. (\<forall>z. s \<in> P' z \<longrightarrow> t \<in> Q z) \<longrightarrow> (\<forall>z. s \<in> P z \<longrightarrow> t \<in> Q z) \<Longrightarrow> \<forall>z. ht (P z) (apre (P' z) x) (Q z)"
+  by (force simp add: apre_def seq_def ht_def)
 
-lemma hl_apre3: "\<forall>z. ht (P' z) x (Q' z) \<Longrightarrow> \<forall>s t. (\<forall>z. s \<in> P' z \<longrightarrow> t \<in> Q' z) \<longrightarrow> (\<forall>z. s \<in> P z \<longrightarrow> t \<in> Q z) \<Longrightarrow> ht (P z) x (Q z)"
-  apply (simp add: apre_def seq_def ht_def)
-  apply auto
-  by force
-
-lemma hl_2: "P \<subseteq> {s. (\<exists>z. s \<in> P' z \<and> Q' z \<subseteq> Q)} \<Longrightarrow> \<forall>z. ht (P' z) x (Q' z) 
-  \<Longrightarrow> ht P x Q"
-sorry
+lemma hl_apre_kleymann: "ht P' x Q \<Longrightarrow> \<forall>s t. (s \<in> P' \<longrightarrow> t \<in> Q) \<longrightarrow> (s \<in> P \<longrightarrow> t \<in> Q) \<Longrightarrow> ht P (apre P' x) Q"
+  by (force simp add: apre_def seq_def ht_def)
+                                                                               
+lemma hl_apost_classic [hl_rules]: "Q' \<le> Q \<Longrightarrow> ht P x Q' \<Longrightarrow> ht P (apost x Q') Q"
+  by (hoare simp: apost_def hl_rules: hl_apre_kleymann) force
   
-lemma hl_apost [hl_rules]: "Q' \<le> Q \<Longrightarrow> ht P x Q' \<Longrightarrow> ht P (apost x Q') Q"
-  by (auto simp: apost_def le_fun_def intro!: hl_seq hl_apre hl_skip)
-  
-lemma hl_aprog [hl_rules]: "P \<le> P' \<Longrightarrow> Q' \<le> Q \<Longrightarrow> ht P' x Q' \<Longrightarrow> ht P (aprog P' x Q') Q"
+lemma hl_aprog_classic : "P \<le> P' \<Longrightarrow> Q' \<le> Q \<Longrightarrow> ht P' x Q' \<Longrightarrow> ht P (aprog P' x Q') Q"
   by (hoarerule simp: aprog_def first: hl_classic)
 
+(***********************************************************************************************)
+
+text {* When using hoare, rules should be applied in the following order *}
+
+declare hl_split
+  hl_local_inv [hl_rules]
+  hl_loc_block [hl_rules]
+  hl_fun_block [hl_rules]
+  hl_block [hl_rules]
+
+declare subst_def [simp]
 
 end
