Syntax.thy
@@ -5,55 +5,128 @@ begin
 (* Syntax of the While language *)
 
 syntax
-  "_quote" :: "'a \<Rightarrow> ('s \<Rightarrow> 'a)" ("(\<guillemotleft>_\<guillemotright>)" [0] 1000)
-  "_antiquote" :: "('s \<Rightarrow> 'a) \<Rightarrow> 's" ("`_" [1000] 1000) 
-  "_quote2" :: "'a \<Rightarrow> ('s \<Rightarrow> 'a)" ("(\<guillemotleft>2_\<guillemotright>)" [0] 1000)
-  "_antiquote2" :: "('s \<Rightarrow> 'a) \<Rightarrow> 's" ("`2_" [1000] 1000)
-  "_subst" :: "'s set \<Rightarrow> 'a \<Rightarrow> idt \<Rightarrow> 's set" ("_[_'/`_]" [1000] 999)
-  "_assign" :: "idt \<Rightarrow> 'a \<Rightarrow> 's rel" ("(`_ :=/ _)" [0, 65] 62)
-  "_cond" :: "'s set \<Rightarrow> 's rel \<Rightarrow> 's rel \<Rightarrow> 's rel" ("(0if _ then//  _//else//  _//fi)" [0,0,0] 62)
-  "_cond_skip" :: "'s set \<Rightarrow> 's rel \<Rightarrow> 's rel" ("(0if _//then _//fi)" [0,0] 62)
-  "_while" :: "'s set \<Rightarrow> 's rel \<Rightarrow> 's rel" ("(0while  _//do  _//od)" [0, 0] 62)
-  "_awhile" :: "'s set \<Rightarrow> 's set \<Rightarrow> 's rel \<Rightarrow> 's rel" ("(0while _//inv  _//do _//od)" [0, 0, 0] 62)
-  "_awhile_aux" :: "'s set \<Rightarrow> 'v \<Rightarrow> 's set \<Rightarrow> 's rel \<Rightarrow> 's rel" ("(0while _//inv _. _//do _//od)" [0, 0, 0] 62)
-  "_local" :: "idt \<Rightarrow> 'b \<Rightarrow> 'a rel \<Rightarrow> 'a rel" ("local `_ := _ in _ end" [0, 65, 55] 62)
-  "_local2" :: "idt \<Rightarrow> 'a rel \<Rightarrow> 'a rel" ("local `_ in _ end" [0, 55] 62)
-  "_locals" :: "idts \<Rightarrow> 's rel \<Rightarrow> 's rel" ("locals _ in _ end" [0, 55] 62)
-  "_proc" :: "idt \<Rightarrow> 'a rel \<Rightarrow> idt \<Rightarrow> 'b \<Rightarrow> 'a rel" ("`_ := call _ `_ : _" [0, 65, 55] 62)
-  "_rec" :: "'s rel \<Rightarrow> 's rel \<Rightarrow> 's rel" ("rec _ in _ end" [0, 55] 62)
-  "_apre" :: "'s set \<Rightarrow> 's rel \<Rightarrow> 's rel" ("\<lbrace> _ \<rbrace> _" [0, 62] 62)
-  "_apre_aux" :: "'v \<Rightarrow> ('v \<Rightarrow> 's set) \<Rightarrow> 's rel \<Rightarrow> 's rel" ("\<lbrace> _ . _ \<rbrace> _" [0, 0, 62] 62)
-  "_call" :: "idt \<Rightarrow> ('s rel \<times> ('s \<Rightarrow> 'v)) \<Rightarrow> 's rel" ("`_ := call _ " [0, 65] 62)
+  "_quote"      :: "'a \<Rightarrow> ('s \<Rightarrow> 'a)"                       ("(\<guillemotleft>_\<guillemotright>)" [0] 1000)
+  "_antiquote"  :: "('s \<Rightarrow> 'a) \<Rightarrow> 's"                       ("`_" [1000] 1000) 
+  "_quote2"     :: "'a \<Rightarrow> ('s \<Rightarrow> 'a)"                       ("(\<guillemotleft>2_\<guillemotright>)" [0] 1000)
+  "_antiquote2" :: "('s \<Rightarrow> 'a) \<Rightarrow> 's"                       ("`2_" [1000] 1000)
+
+  "_subst"      :: "'s set \<Rightarrow> 'v \<Rightarrow> idt \<Rightarrow> 's set"          ("_[_'/`_]" [1000] 999)
+  "_assign"     :: "idt \<Rightarrow> 'a \<Rightarrow> 's rel"                    ("(`_ :=/ _)" [0, 65] 62)
+
+  "_cond"       :: "'s set \<Rightarrow> 's rel \<Rightarrow> 's rel \<Rightarrow> 's rel"   ("(0if _ then//  _//else//  _//fi)" [0,0,0] 62)
+  "_cond_skip"  :: "'s set \<Rightarrow> 's rel \<Rightarrow> 's rel"             ("(0if _//then _//fi)" [0,0] 62)
+  "_while"      :: "'s set \<Rightarrow> 's rel \<Rightarrow> 's rel"             ("(0while  _//do  _//od)" [0, 0] 62)
+  "_awhile"     :: "'s set \<Rightarrow> 's set \<Rightarrow> 's rel \<Rightarrow> 's rel"   ("(0while _//inv _//do// _//od)" [0, 0, 0] 62)
+
+  "_apre"       :: "'s set \<Rightarrow> 's rel \<Rightarrow> 's rel"               ("\<lbrace> _ \<rbrace>// _" [0, 62] 62)
+  "_apre_aux"   :: "'v \<Rightarrow> ('v \<Rightarrow> 's set) \<Rightarrow> 's rel \<Rightarrow> 's rel" ("\<lbrace> _ . _ \<rbrace> _" [0, 0, 62] 62)
+
+  "_proc"       :: "'s rel \<Rightarrow> 's rel"                        ("begin// _//end")
+  "_fun"        :: "'s rel \<Rightarrow> 'a \<Rightarrow> ('s rel \<times> 'a)"           ("begin// _// return `_//end")
+  "_local"      :: "idt \<Rightarrow> 'b \<Rightarrow> 'a rel \<Rightarrow> 'a rel"           ("(0local `_ := _ in// _//end)" [0, 65, 55] 62)
+  "_call"       :: "idt \<Rightarrow> ('s rel \<times> ('s \<Rightarrow> 'v)) \<Rightarrow> 's rel"  ("`_ := call (0_) " [0, 65] 62)
+
+  "_rec"        :: "'s rel \<Rightarrow> 's rel \<Rightarrow> 's rel"               ("(0rec _ in// _//end)" [0, 55] 62)
+
+  "_ht"         :: "'s set \<Rightarrow> 's rel \<Rightarrow> 's set \<Rightarrow> bool"       ("\<turnstile> \<lbrace> _ \<rbrace>// _// \<lbrace> _ \<rbrace>" [0, 55, 0] 50)
+  "_ht_aux"     :: "'v \<Rightarrow> 's set \<Rightarrow> 's rel \<Rightarrow> 's set \<Rightarrow> bool" ("\<turnstile> \<lbrace> _ . _ \<rbrace>// _// \<lbrace> _ \<rbrace>" [0, 55, 0] 50)
+
+
 
 ML {*
-fun quote_tr [t] = Syntax_Trans.quote_tr @{syntax_const "_antiquote"} t
-    | quote_tr ts = raise TERM ("quote_tr", ts)
-fun quote2_tr [t] = Syntax_Trans.quote_tr @{syntax_const "_antiquote2"} t
-    | quote2_tr ts = raise TERM ("quote2_tr", ts)
+  fun quote_tr [t] = Syntax_Trans.quote_tr @{syntax_const "_antiquote"} t
+      | quote_tr ts = raise TERM ("quote_tr", ts)
+  fun quote2_tr [t] = Syntax_Trans.quote_tr @{syntax_const "_antiquote2"} t
+      | quote2_tr ts = raise TERM ("quote2_tr", ts)
 *}
 
 parse_translation {*
-  [(@{syntax_const "_quote"}, K quote_tr), (@{syntax_const "_quote2"}, K quote2_tr)]
+  [(@{syntax_const "_quote"}, K quote_tr), 
+  (@{syntax_const "_quote2"}, K quote2_tr)]
 *}
 
-abbreviation id2 :: "'s \<Rightarrow> 's \<Rightarrow> 's" where
-  "id2 \<equiv> \<lambda>s t. s"
-
 translations
-  "p [t/`u]" == "CONST Collect \<guillemotleft> `(_update_name u (\<lambda>_. t)) \<in> p \<guillemotright>"
-  "`u := t" => "CONST to_rel \<guillemotleft>`(_update_name u (\<lambda>_. t))\<guillemotright>"
-  "if b then x else y fi" => "CONST cond (CONST Collect \<guillemotleft>b\<guillemotright>) x y"
-  "if b then x fi" == "if b then x else skip fi"
-  "while b inv i do x od" => "CONST awhile (CONST Collect \<guillemotleft>i\<guillemotright>) (CONST Collect \<guillemotleft>b\<guillemotright>) x"
+  "p [t/`u]"                == "_update_name u (\<lambda>_. t) \<in> p"
+  "`u := t"                 == "CONST assign(_update_name u) \<guillemotleft>t\<guillemotright>"
+
+  "if b then x else y fi"   => "CONST cond (CONST Collect \<guillemotleft>b\<guillemotright>) x y"
+  "if b then x fi"          == "if b then x else skip fi"
+  "while b do x od"         == "CONST cwhile (CONST Collect \<guillemotleft>b\<guillemotright>) x"
+  "while b inv i do x od"   == "CONST awhile (CONST Collect \<guillemotleft>i\<guillemotright>) (CONST Collect \<guillemotleft>b\<guillemotright>) x"
+
+  "\<lbrace> p \<rbrace> x"                 == "CONST apre (CONST Collect \<guillemotleft>p\<guillemotright>) x"
+  "\<lbrace> u . p \<rbrace> x"             => "CONST apre (CONST Collect \<guillemotleft>p\<guillemotright>) x"
+
+  "begin x end"             => "x"
+  "begin x return `z end"   == "CONST fun_block x z"
+  "local `u := t in x end"  => "CONST loc_block (_update_name u) \<guillemotleft>`u\<guillemotright> \<guillemotleft>t\<guillemotright> x"
+  "`z := call R"            => "CONST fun_call (_update_name z) R"
+
+  "(rec f in x end) z"          => "CONST lfp (%f z. x z)"
+
+  "\<turnstile> \<lbrace> p \<rbrace> x \<lbrace> q \<rbrace>"         => "CONST ht (CONST Collect \<guillemotleft>p\<guillemotright>) x (CONST Collect \<guillemotleft>q\<guillemotright>)"
+  "\<turnstile> \<lbrace> u . p \<rbrace> x \<lbrace> q \<rbrace>"     => "\<forall>u. CONST ht (CONST Collect \<guillemotleft>p\<guillemotright>) x (CONST Collect \<guillemotleft>q\<guillemotright>)"
+  
+
+(* Pretty printing *)
+
+syntax ("" output)
+  "_assert"    :: "'s \<Rightarrow> 's set"                             ("[_]" [0] 1000)
+  "_seq"       :: "'s rel \<Rightarrow> 's rel \<Rightarrow> 'a rel"               ("_;// _" [59, 59] 60 )
+  "_ht"        :: "'s set \<Rightarrow> 's rel \<Rightarrow> 's set \<Rightarrow> bool"       ("\<turnstile> \<lbrace> _ \<rbrace>// _// \<lbrace> _ \<rbrace>" [0, 55, 0] 50)
+
+ML {*
+  fun quote_tr' f (t :: ts) =
+          Term.list_comb (f $ Syntax_Trans.quote_tr' @{syntax_const "_antiquote"} t, ts)
+      | quote_tr' _ _ = raise Match;
+
+  val assert_tr' = quote_tr' (Syntax.const @{syntax_const "_assert"});
+
+  fun subst_tr' (p :: x :: ts) = (quote_tr' (Syntax.const @{syntax_const "_subst"} $ p) ts) $ Syntax_Trans.update_name_tr' x
+    | subst_tr' _ = raise Match;
+
+  fun assign_tr' (x :: ts) =  quote_tr' (Syntax.const @{syntax_const "_assign"} $ Syntax_Trans.update_name_tr' x) ts
+    | assign_tr' _ = raise Match;
+
+  fun local_tr' [x, _,  t, y] = (quote_tr' (Syntax.const @{syntax_const "_local"} $ Syntax_Trans.update_name_tr' x) [t]) $ y
+    | local_tr' _ = raise Match;
+
+  fun call_tr' [z, f] = Syntax.const @{syntax_const "_call"} $ Syntax_Trans.update_name_tr' z $ f
+    | call_tr' _ = raise Match;
+
+  fun print_tr' name [x, y, z] = Syntax.const name $ x $ y $ z
+    | print_tr' name [x, y] = Syntax.const name $ x $ y
+    | print_tr' name [x] = Syntax.const name $ x
+    | print_tr' _ _ = raise Match;
+
+*}
+
+print_translation {*
+  [
+  (@{const_syntax Collect}, K assert_tr'),
+  (@{const_syntax assign}, K assign_tr'),
+  (@{const_syntax subst}, K subst_tr'),
+
+  (@{const_syntax seq}, K (print_tr' @{syntax_const "_seq"})),
+  (@{const_syntax cond}, K (print_tr' @{syntax_const "_cond"})),
+  (@{const_syntax awhile}, K (print_tr' @{syntax_const "_awhile"})),
+
+  (@{const_syntax apre}, K (print_tr' @{syntax_const "_apre"})),
+
+  (@{const_syntax loc_block}, K local_tr'),
+  (@{const_syntax fun_call}, K call_tr'),
+
+  (@{const_syntax ht}, K (print_tr' @{syntax_const "_ht"}))
+  ]
+*}
+
+(*
+
+  "_local2"     :: "idt \<Rightarrow> 'a rel \<Rightarrow> 'a rel" ("local `_ in _ end" [0, 55] 62)
+  "_locals"     :: "idts \<Rightarrow> 's rel \<Rightarrow> 's rel" ("locals _ in _ end" [0, 55] 62)
+
   "while b inv u. i do x od" => "CONST awhile (%u. CONST Collect \<guillemotleft>i\<guillemotright>) (CONST Collect \<guillemotleft>b\<guillemotright>) x"
-  "local `u := t in x end" => "CONST block (CONST id) (`u := t; x) (\<guillemotleft>2 \<guillemotleft>`(_update_name u (\<lambda>_. `2 u))\<guillemotright> \<guillemotright>) (\<guillemotleft>2 \<guillemotleft> skip \<guillemotright>\<guillemotright>)"
   "local `u in x end" => "CONST block (CONST id) x (\<guillemotleft>2 \<guillemotleft>`(_update_name u (\<lambda>_. `2 u))\<guillemotright> \<guillemotright>) (\<guillemotleft>2 \<guillemotleft> skip \<guillemotright>\<guillemotright>)"
-  "\<lbrace> p \<rbrace> x" => "CONST apre (CONST Collect \<guillemotleft>p\<guillemotright>) x"
-  "\<lbrace> u . p \<rbrace> x" => "CONST apre (CONST Collect \<guillemotleft>p\<guillemotright>) x"
-  "rec f in x end" => "CONST lfp (%f. x)"
-  " `z := call R" => "CONST block (CONST id) (CONST fst R) (CONST id2) (\<guillemotleft> \<guillemotleft>2 `z := `2 (CONST snd R) \<guillemotright>\<guillemotright>)"
-  (*"`u := call R `v : t" => "CONST block (\<guillemotleft>`(_update_name v (\<lambda>_. t))\<guillemotright>) R (\<guillemotleft> \<guillemotleft>2 \<guillemotleft>`(_update_name v (\<lambda>_. `2 v))\<guillemotright> \<guillemotright> \<guillemotright>) (\<guillemotleft>2 \<guillemotleft> `u := `2 v \<guillemotright>\<guillemotright>)"
-*)(* Syntax of Hoare logic *)
 
 ML {*
 
@@ -90,15 +163,6 @@ parse_translation {*
   [(@{syntax_const "_locals"}, K locals_tr)]
 *}
 
-
-syntax
-  "_ht" :: "'s set \<Rightarrow> 's rel \<Rightarrow> 's set \<Rightarrow> bool" ("\<turnstile> \<lbrace> _ \<rbrace>// _// \<lbrace> _ \<rbrace>" [0, 55, 0] 50)
-  "_ht_aux" :: "'v \<Rightarrow> 's set \<Rightarrow> 's rel \<Rightarrow> 's set \<Rightarrow> bool" ("\<turnstile> \<lbrace> _ . _ \<rbrace>// _// \<lbrace> _ \<rbrace>" [0, 55, 0] 50)
-
-translations
-  "\<turnstile> \<lbrace> p \<rbrace> x \<lbrace> q \<rbrace>" == "CONST ht (CONST Collect \<guillemotleft>p\<guillemotright>) x (CONST Collect \<guillemotleft>q\<guillemotright>)"
-  "\<turnstile> \<lbrace> u . p \<rbrace> x \<lbrace> q \<rbrace>" => "\<forall>u. CONST ht (CONST Collect \<guillemotleft>p\<guillemotright>) x (CONST Collect \<guillemotleft>q\<guillemotright>)"
-
-
+*)
 
 end
